Qsort/Monadic/QpartitionAltHoles.lean
@@ -1,0 +1,262 @@
+import Std.Tactic.Do
+import Qsort.AuxLemmas
+import Qsort.Monadic.Aux
+import Qsort.Monadic.Theory
+import Qsort.SDo.VCGen
+
+set_option mvcgen.warning false
+set_option pp.showLetValues true
+
+open Std.Do
+open List
+
+namespace Monadic.Qpartition
+
+@[inline] def qpartition (x1 x2 x3 x4 x5 x6 x7 x8 x9 x10 x11 x12 x13 : HP Nat → HP Nat → Nat) (x14 : Nat) (x15 : HP Nat → Nat) 
+    (lt : α → α → Bool) (lo hi : Nat) (hlo : lo < n) (hhi: hi < n) (hle : lo ≤ hi) :
+    StateM (ST α n) $ {pivot : Nat // lo ≤ pivot ∧ pivot ≤ hi} := do
+  qp_prep lt lo hi hlo hhi
+  let mut i : Nat := x14
+  let mut j : Nat := x15 i
+  for _ in [x11 i j:x12 i j] do
+    -- FIXME need assertions in place of `sorry`s
+    let xs := (← get).xs -- FIXME
+    if lt (xs.get (x1 i j) sorry) (xs.get (x2 i j) sorry) then
+      swap (x9 i j) (x10 i j) sorry sorry
+      i := x5 i j
+      j := x6 i j
+    else
+      i := x7 i j
+      j := x8 i j
+  swap (x3 i j) (x4 i j) sorry sorry
+  pure ⟨x13 i j, sorry, sorry⟩
+
+variable {lt : α → α → Bool} 
+
+theorem test (a b : Nat) (h : a < b) (h' : b ≤ a) : False := by omega
+
+namespace qpartition
+
+-- set_option trace.Elab.Tactic.Do.vcgen true in
+theorem sorted 
+   (le_asymm : ∀ {{a b}}, lt a b → ¬lt b a)
+   (le_trans : ∀ {{a b c}}, ¬lt a b → ¬lt b c → ¬lt a c)
+   (lo hi : Nat) (hlo : lo < n := by omega) (hhi : hi < n := by omega) (hle : lo ≤ hi)
+   :
+   ∃ x1 x2 x3 x4 x5 x6 x7 x8 x9 x10 x11 x12 x13 x14 x15,
+   ⦃fun s => ⌜s.xs = xs⌝⦄
+   qpartition x1 x2 x3 x4 x5 x6 x7 x8 x9 x10 x11 x12 x13 x14 x15 lt lo hi hlo hhi hle
+   ⦃⇓ pivot s => ⌜
+     (∀ (x : Nat), lo ≤ x → x < pivot.1 → (h : x < n) → ¬lt ((s.xs).get pivot.1 (by omega)) ((s.xs).get x h)) ∧
+     (∀ (x : Nat), pivot.1 < x → x ≤ hi → (h : x < n) → ¬lt ((s.xs).get x h) ((s.xs).get pivot.1 (by omega))) ∧
+     Stable s.xs xs lo hi hlo hhi
+   ⌝⦄ := by
+  exists? mvar1
+  exists? mvar2
+  exists? mvar3
+  exists? mvar4
+  exists? mvar5
+  exists? mvar6
+  exists? mvar7
+  exists? mvar8
+  exists? mvar9
+  exists? mvar10
+  exists? mvar11
+  exists? mvar12
+  exists? mvar13
+  exists? mvar14
+  exists? mvar15
+
+  mvar mvar01 : HP Nat → HP Nat → Nat -- loop invariant mvars
+  mvar mvar02 : HP Nat → HP Nat → Nat
+  mvar mvar03 : HP Nat → HP Nat → Nat
+  mvar mvar04 : HP Nat → HP Nat → Nat
+
+  -- FIXME could `mvcgen` attempt to auto-unfold definitions that it doesn't have a spec for?
+  unfold qpartition
+  smvcgen [qp_prep.stable] invariants
+  . ⇓ t => fun s =>
+      let sp := t.1;
+      let ⟨i, j⟩ := t.2;
+      ⌜(∀ (x : Nat), (?mvar03 i j) ≤ x → x < i → (hx : x < n) → (hm : (?mvar01 i j) < n) → ¬ lt ((s.xs).get (?mvar01 i j) hm) ((s.xs).get x hx))
+      ∧
+      (∀ (x : Nat), i ≤ x → x < j → (hx : x < n) → (hm : (?mvar02 i j) < n) → ¬ lt ((s.xs).get x hx) ((s.xs).get (?mvar02 i j) hm))
+      ∧
+      (j = lo + sp.prefix.length)
+      ∧
+      ((?mvar04 i j) ≤ i ∧ i ≤ j)
+      ∧
+      (Stable s.xs xs lo hi hlo hhi)⌝
+
+  case vc5.post.success.post.success =>
+    rename_i r _ h
+
+    simp only [lists, arith] at *
+
+    rcases h with ⟨hl, hr, hj, _,  _⟩ -- FIXME
+    rcases r with ⟨i, j⟩
+    simp only at * -- FIXME
+    
+    and_intros
+    intro x
+    intros
+    inst mvar3
+      rw [Vector.swap.get_left]
+    ite x rw [Vector.swap.get_right]
+    apply hl
+    inst' mvar03 apply Nat.succ_le_of_lt
+    apply Nat.succ_le_of_lt
+    nthassumption mvar03_0 2
+
+    rw [Vector.swap.get_other]
+    inst mvar4 apply hl
+    inst mvar03 assumption
+    inst mvar13 assumption
+    omega
+    rotate_left
+
+    intros x _ _ _ -- FIXME
+    rw [Vector.swap.get_left]
+    ite x rw [Vector.swap.get_right]
+    inst mvar02 apply hr
+    omega
+    rotate_left 1
+    . rw [Vector.swap.get_other]
+      apply hr
+      omega
+      ite j 
+        apply lt_of_ne
+        assumption
+        apply ne_symm
+        inst mvar01 assumption
+      . false_or_by_contra -- FIXME
+        apply h
+
+        apply eq_comm
+        apply eq_trans
+        exact hj
+        inst mvar11 inst mvar12 apply add_sub
+        assumption
+      omega
+      omega
+    rotate_right
+    ite j assumption
+    . false_or_by_contra -- FIXME
+      apply h
+
+      omega
+
+    . rename_i h
+      rcases h
+      apply Vector.swap.stable
+      omega
+      inst mvar04 assumption
+      omegas
+
+    omega
+
+  sorries
+  . rename_i pref cur suff h' _ _ h _
+    -- FIXME
+    have hrng_dec_sz : (pref ++ cur :: suff).length = hi - lo := by
+      rw [← h']
+      simp only [lists, arith]
+    simp only [lists, arith] at *
+    rcases h with ⟨hl, hr, hj, _,  _⟩
+
+    and_intros
+    apply pred_range_extend
+
+    intros x
+    intros
+    rw [Vector.swap.get_other]
+    rw [Vector.swap.get_other]
+    apply hl
+    assumption
+    assumption
+    apply ne_of_lt
+    nthassumption mvar9 3
+    rotate_left 3 -- FIXME tactic to collectively defer all remaining goals in a .focus block not solved by `omega`
+
+    inst mvar5 apply pred_range_single
+    intros
+    rw [Vector.swap.get_left]
+    rw [Vector.swap.get_other]
+    apply le_asymm
+    omegas
+    inst mvar1 inst mvar2 assumption
+    rotate_left 1 -- FIXME
+
+    apply pred_range_extend
+    intros x
+    intros
+    . rw [Vector.swap.get_other]
+      rw [Vector.swap.get_other]
+      omegas
+      apply hr
+      rename_i hp _ _ _ _
+      omegas
+      rotate_right 1
+      apply ne_of_lt
+      nthassumption mvar10 3
+      omegas
+    . inst mvar6 apply pred_range_single
+      intros
+      rw [Vector.swap.get_right]
+      rw [Vector.swap.get_other]
+      omegas
+      apply hr
+      omegas
+    omegas
+    . apply Vector.swap.stable
+      omegas
+
+  . rename_i pref cur suff h' _ _ h _ 
+    -- FIXME
+    have hrng_dec_sz : (pref ++ cur :: suff).length = hi - lo := by
+      rw [← h']
+      simp only [lists, arith]
+    simp only [lists, arith] at *
+    rcases h with ⟨hl, hr, hj, _,  _⟩
+    
+    and_intros
+    omegas
+    inst mvar7 assumption
+    apply pred_range_extend
+    . intros x
+      intros
+      apply hr
+      omegas
+    inst mvar8 apply pred_range_single
+    intros
+    omegas
+
+  . rename_i h' _ _ h
+    rw [h'] at h
+    simp only [lists, arith] at *
+
+    and_intros
+
+    intros _ _ hm
+    intros
+    have := Nat.not_le_of_lt hm
+    false_or_by_contra
+    apply this
+    inst mvar14 assumption
+
+    intros _ _ hm
+    intros
+    have := Nat.not_le_of_lt hm
+    false_or_by_contra
+    apply this
+    inst mvar15 assumption
+
+    omegas
+
+-- theorem perm {lo : Fin n} {hi : Fin n} (hle : lo ≤ hi := by omega) :
+--    ∃ x1 x2 x3 x4,
+--    ⦃⌜#gxs = xs⌝⦄
+--    qpartition x1 x2 x3 x4 lt lo hi hle
+--    ⦃⇓ pivot => ⌜Perm (#gxs) xs⌝⦄ := by
+--   sorry
+end qpartition
